@prefix rdf: <http://www.w3.org/1999/02/22-rdf-syntax-ns#> .
@prefix rdfs: <http://www.w3.org/2000/01/rdf-schema#> .
@prefix owl: <http://www.w3.org/2002/07/owl#> .
@prefix xsd: <http://www.w3.org/2001/XMLSchema#> .
@prefix skos: <http://www.w3.org/2004/02/skos/core#> .
@prefix dcterms: <http://purl.org/dc/terms/> .
@prefix foaf: <http://xmlns.com/foaf/0.1/>.
@prefix time: <http://www.w3.org/2006/time#> .

@prefix schema: <http://schema.org/> .

@prefix sosa: <http://www.w3.org/ns/sosa/> .
@prefix sosa-core: <http://www.w3.org/ns/sosa/core/> .
@prefix sosa-obs: <http://www.w3.org/ns/sosa/obs/> .


sosa-obs: 
  a owl:Ontology ;
  dcterms:title "Sensor, Observation, Sample, and Actuator (SOSA) Ontology - actuation module"@en ;
  dcterms:description "Observation classes and properties for the SSN Ontology."@en ;
  dcterms:creator [ a foaf:Agent ; foaf:name "W3C/OGC Spatial Data on the Web Working Group"@en ] ;
  dcterms:rights "Copyright 2024 W3C/OGC." ;
  dcterms:license <http://www.w3.org/Consortium/Legal/2015/copyright-software-and-document> ;
  dcterms:license <http://www.opengeospatial.org/ogc/Software> ;
  dcterms:created "2024-02-02"^^xsd:date ;
  owl:imports sosa-core: ;
  .

sosa:ObservableProperty 
  a owl:Class ;
  rdfs:label "Observable Property"@en ;
  skos:definition "An observable quality (property, characteristic) of a FeatureOfInterest."@en ;
  rdfs:comment "'Observable' means that the value may be determined through an act of Observation using an ObservationProcedure applied by a Sensor or Observer. This can be contrasted with properties whose value is assigned by some authority (e.g. price, ownership), or whose value is a consequence of some other values (e.g. rank). "@en ;
  skos:example "The height of a tree, the depth of a water body, or the temperature of a surface. "@en ;
  rdfs:isDefinedBy sosa-obs: .

sosa:ObservingProcedure 
  a owl:Class ;
  rdfs:label "Observing Procedure"@en ;
  skos:definition "The description of steps performed in order to determine the value of an ObservableProperty by an Observer."@en ;
  skos:example "A workflow, protocol, plan, algorithm, or computational method specifying how to make an observation; the description of the process utilized by an observer. This could be a chemical analysis method, a protocol for measuring an object, but could also be a checklist utilized by a human observer during a biodiversity campaign."@en ;
  skos:note "The observing procedure cannot describe a sensor instance, but it can describe the sensor type."@en ;
  rdfs:isDefinedBy sosa-obs: .

sosa:Sensor 
  a owl:Class ;
  rdfs:label "Sensor or Observer"@en ;
  skos:altLabel "Observer"@en ;
  skos:prefLabel "Sensor"@en ;
  skos:definition """An identifiable entity that can generate Observations pertaining to an ObservableProperty by implementing an ObservingProcedure. Device, agent (including humans), or software (simulation) involved in, or implementing, a Procedure. Sensors respond to a stimulus, e.g., a change in the environment, or input data composed from the results of prior Observations, and generate a Result. Sensors can be hosted by Platforms."""@en ;
  skos:example "Accelerometers, gyroscopes, barometers, magnetometers, and so forth are Sensors that are typically mounted on a modern smartphone (which acts as Host or Platform). Other examples of Sensors include the human eyes."@en ;
  skos:note "Different Sensors can follow the same (reusable) observing Procedure for the creation of different Observations."@en ;
  skos:note "The Sensor is the entity instance, not the entity type. Pertaining to sensors, the Sensor would reference the explicit sensor, while the Procedure would reference the methodology utilized by that sensor type;"@en ;
  skos:note "A Sensor can be hosted by one or more Platform."@en ;
  skos:note "The Sensor is an instance of a sensor, instrument, implementation of an algorithm, or a being such as a person."@en ;
  rdfs:comment "Device, agent (including humans), or software (simulation) involved in, or implementing, a Procedure. Sensors respond to a stimulus, e.g., a change in the environment, or input data composed from the results of prior Observations, and generate a Result. Sensors can be hosted by Platforms."@en ;
  skos:example "Accelerometers, gyroscopes, barometers, magnetometers, and so forth are Sensors that are typically mounted on a modern smart phone (which acts as Platform). Other examples of sensors include the human eyes."@en ;
  skos:scopeNote "The UML class 'Observer' from ISO 19156:2023 is implemented in SOSA by the OWL/RDFS class 'Sensor'. The class name 'Sensor' is preferred for backward compatibility with existing SOSA deployments. " ;
  rdfs:isDefinedBy sosa-obs: .

sosa:observes 
  a owl:ObjectProperty ;
  rdfs:label "observes"@en ;
  skos:definition "Relation between a Sensor and an ObservableProperty that it is capable of sensing."@en ;
  rdfs:comment "Relation between a Sensor and an ObservableProperty that it is capable of sensing."@en ;
  schema:domainIncludes sosa:Sensor ;
  schema:rangeIncludes sosa:ObservableProperty ;
  owl:inverseOf sosa:isObservedBy ;
  rdfs:isDefinedBy sosa-obs: .

sosa:isObservedBy 
  a owl:ObjectProperty ;
  rdfs:label "is observed by"@en ;
  skos:definition "Relation between an ObservableProperty and the Sensor able to observe it."@en ;
  rdfs:comment "Relation between an ObservableProperty and the Sensor able to observe it."@en ;
  schema:domainIncludes sosa:ObservableProperty ;
  schema:rangeIncludes sosa:Sensor ;
  owl:inverseOf sosa:observes ;
  rdfs:isDefinedBy sosa-obs: .

sosa:Observation 
  a owl:Class ;
  rdfs:label "Observation"@en ;
  skos:definition "Act of carrying out an (Observation) Procedure to estimate or calculate a value of a property of a FeatureOfInterest. Links to a Sensor to describe what made the Observation and how; links to an ObservableProperty to describe what the result is an estimate of, and to a FeatureOfInterest to detail what entity that property was associated with."@en ;
  rdfs:comment """An Observation concerns a single ObservableProperty of a single FeatureOfInterest. 
  Observations of multiple properties, or other combinations of Observations, may be described in an ObservationCollection. 
  
  Alternatively, applications may choose to encapsulate complexity by defining a complex property with multiple individual components, and a corresponding complex result (e.g. a vector). 
  This approach is not prohibited by the SSN Ontology, but the details are beyond the scope of SSN."""@en ;
  skos:example "The activity of estimating the intensity of an Earthquake using the Mercalli intensity scale is an Observation as is measuring the moment magnitude, i.e., the energy released by said earthquake."@en ;
  rdfs:isDefinedBy sosa-obs: .

sosa:madeObservation 
  a owl:ObjectProperty ;
  rdfs:label "made observation"@en ;
  skos:definition "Relation between a Sensor and an Observation made by the Sensor."@en ;
  rdfs:comment "Relation between a Sensor and an Observation made by the Sensor."@en ;
  schema:domainIncludes sosa:Sensor ;
  schema:rangeIncludes sosa:Observation ;
  owl:inverseOf sosa:madeBySensor ;
  rdfs:isDefinedBy sosa-obs: .

sosa:madeBySensor 
  a owl:ObjectProperty ;
  rdfs:label "made by sensor or observer"@en ;
  skos:definition "Relation between an Observation and the Sensor or Observer which made the Observation."@en ;
  rdfs:comment "Relation between an Observation and the Sensor or Observer which made the Observation."@en ;
  schema:domainIncludes sosa:Observation ;
  schema:domainIncludes sosa:ObservationCollection ;
  schema:rangeIncludes sosa:Sensor ;
  owl:inverseOf sosa:madeObservation ;
  rdfs:isDefinedBy sosa-obs: .

sosa:observedProperty 
  a owl:ObjectProperty ;
  rdfs:label "observed property"@en ;
  skos:definition "Relation linking an Observation to the property that was observed. The ObservableProperty should be a property of the FeatureOfInterest (linked by hasFeatureOfInterest) of this Observation."@en ;
  rdfs:comment "Relation linking an Observation to the property that was observed. The ObservableProperty should be a property of the FeatureOfInterest (linked by hasFeatureOfInterest) of this Observation."@en ;
  schema:domainIncludes sosa:Observation ;
  schema:domainIncludes sosa:ObservationCollection ;
  schema:rangeIncludes sosa:ObservableProperty ;
  rdfs:isDefinedBy sosa-obs: .

sosa:madeBySensor 
  a owl:ObjectProperty ;
  rdfs:label "made by sensor or observer"@en ;
  skos:definition "Relation between an Observation and the Sensor or Observer which made the Observation."@en ;
  rdfs:comment "Relation between an Observation and the Sensor or Observer which made the Observation."@en ;
  schema:domainIncludes sosa:Observation ;
  schema:domainIncludes sosa:ObservationCollection ;
  schema:rangeIncludes sosa:Sensor ;
  owl:inverseOf sosa:madeObservation ;
  rdfs:isDefinedBy sosa-obs: .

sosa:relatedObservation 
  a owl:ObjectProperty ;
  rdfs:label "related observation"@en ;
  skos:definition "Relation to an Observation."@en ;
  schema:domainIncludes sosa:Actuation ;
  schema:domainIncludes sosa:ActuationCollection ;
  schema:domainIncludes sosa:ObservableProperty ;
  schema:domainIncludes sosa:Observation ;
  schema:domainIncludes sosa:ObservationCollection ;
  schema:domainIncludes sosa:Platform ;
  schema:domainIncludes sosa:Procedure ;
  schema:domainIncludes sosa:Sample ;
  schema:domainIncludes sosa:Sensor ;
  schema:rangeIncludes sosa:Observation ;
  schema:rangeIncludes sosa:ObservationCollection ;
  rdfs:isDefinedBy sosa-obs: .

## Stimulus

sosa:Stimulus 
  a owl:Class ;
  rdfs:label "Stimulus"@en ;
  skos:definition "An event in the real world that 'triggers' the Sensor. The properties associated to the Stimulus may be different to the eventual observed ObservableProperty. It is the event, not the object, that triggers the Sensor."@en ;
  rdfs:comment "An event in the real world that 'triggers' the Sensor. The properties associated to the Stimulus may be different to the eventual observed ObservableProperty. It is the event, not the object, that triggers the Sensor."@en ;
  rdfs:isDefinedBy sosa-obs: .

sosa:wasOriginatedBy 
  a owl:ObjectProperty ;
  rdfs:label "was originated by"@en ;
  skos:definition "Relation between an Observation and the Stimulus that originated it."@en ;
  rdfs:comment "Relation between an Observation and the Stimulus that originated it."@en ;
  schema:domainIncludes sosa:Observation ;
  schema:rangeIncludes sosa:Stimulus ;
  rdfs:isDefinedBy sosa-obs: .

sosa:detects 
  a owl:ObjectProperty ;
  rdfs:label "detects"@en ;
  skos:definition "A relation from a Sensor to the Stimulus that the Sensor detects. The Stimulus itself will be serving as a proxy for some ObservableProperty."@en ;
  rdfs:comment "A relation from a Sensor to the Stimulus that the Sensor detects. The Stimulus itself will be serving as a proxy for some ObservableProperty."@en ;
  schema:domainIncludes sosa:Sensor ;
  schema:rangeIncludes sosa:Stimulus ;
  rdfs:isDefinedBy sosa-obs: .

sosa:isProxyFor 
  a owl:ObjectProperty ;
  rdfs:label "is proxy for"@en ;
  skos:definition "A relation from a Stimulus to the Property that the Stimulus is serving as a proxy for."@en ;
  rdfs:comment "A relation from a Stimulus to the Property that the Stimulus is serving as a proxy for."@en ;
  skos:example "For example, the expansion of quicksilver is a stimulus that serves as a proxy for some temperature property. An increase or decrease in the velocity of spinning cups on a wind sensor is serving as a proxy for the wind speed."@en ;
  schema:domainIncludes sosa:Stimulus ;
  schema:rangeIncludes sosa:ObservableProperty ;
  rdfs:isDefinedBy sosa-obs: .

sosa:resultQuality 
  a owl:ObjectProperty ;
  rdfs:label "observation result quality" ;
  skos:definition "Information pertaining to the data quality of the result." ;
  skos:scopeNote """This instance-specific description complements the description of the observation Procedure, which provides information concerning the quality of all observations using this procedure.""" ; 
  skos:note  """The quality of a result can be assessed following the procedures in the ISO 19157 series. Multiple measures can be provided.""" ;
  skos:note  """dqv:hasQualityMeasurement from the Data Quality Vocabulary is equivalent""" ;
  schema:domainIncludes sosa:Observation ;
  schema:domainIncludes sosa:ObservationCollection ;
  rdfs:isDefinedBy sosa-obs: .

## Observation Collection

sosa:ObservationCollection 
  a owl:Class ;
  rdfs:label "Observation Collection"@en ;
  skos:definition """Collection of one or more observations or observation collections, i.e. collections may be nested. 

  The following Observation properties may appear in an Observation Collection: 
  hasFeatureOfInterest , hasUltimateFeatureOfInterest , usedProcedure , madeBySensor , madeOnPlatform ,  observedProperty , phenomenonTime , resultTime , validTime , hasResult , hasSimpleResult , observationType , hasQualityMeasurement . 
  If it is present, the value of a property summarizes the values of the matching properties of the member observations, where membership is either direct or transitive through one or more member observation collections. 
  The following consistency rules apply with respect to the Observation properties listed above: 
  
  1. Where an individual Observation Collection omits a property, a member Observation (direct or transitive) MAY have any value for that property.

  2. Where an individual Observation Collection has a single value for a property, each member Observation(direct or transitive) MUST have that same value for the property - i.e. the collection is homogeneous in that property.  That property MAY be omitted in any member Observation or Observation Collection.

  3. Where an individual Observation Collection has more than one value for a property, each member Observation (direct or transitive) MUST have a value for that property that matches one of the values for the property in the collection. 
  
  4. Where an individual Observation Collection has a value for a property that is a range or interval, each member Observation (direct or transitive) MUST have a value for that property that matches or falls within that range or interval.

  5. Where an individual Observation Collection has more than one value for a property that is a range or interval, each member Observation (direct or transitive) MUST have a value for that property that either matches or falls within one of those ranges or intervals.
  """@en ;
  skos:note """The members of a collection do not necessarily share a common value for any property. """@en ;
  rdfs:isDefinedBy sosa-obs: .


## End of observation schema
## ---------------------------------------------------- ##
## additional domains and ranges for sosa-core: terms

## Utility terms 

sosa:hasMember 
  schema:domainIncludes sosa:ObservationCollection ;
  schema:rangeIncludes sosa:Observation ;
  schema:rangeIncludes sosa:ObservationCollection ;
  rdfs:isDefinedBy sosa-core: .


## Features of interest and Property

sosa:FeatureOfInterest 
  a owl::Class ;
  rdfs:label "Feature Of Interest"@en ;
  skos:definition "The thing whose property is being estimated or calculated in the course of an Observation to arrive at a Result or whose property is being manipulated by an Actuator, or which is being sampled or transformed in an act of Sampling."@en ;
  rdfs:comment "The thing whose property is being estimated or calculated in the course of an Observation to arrive at a Result or whose property is being manipulated by an Actuator, or which is being sampled or transformed in an act of Sampling."@en ;
  skos:example "When measuring the height of a tree, the height is the observed ObservableProperty, 20m may be the Result of the Observation, and the tree is the FeatureOfInterest. A window is a FeatureOfInterest for an automatic window control Actuator."@en ;
  rdfs:isDefinedBy sosa-core: .

sosa:hasFeatureOfInterest 
  a owl::ObjectProperty ;
  rdfs:label "has feature of interest"@en ;
  skos:definition "A relation between an Observation and the entity whose quality was observed, or between an Actuation and the entity whose property was modified, or between an act of Sampling and the entity that was sampled."@en ;
  skos:scopeNote "Note that this is the _proximate_ feature of interest, which may be a proxy entity such as a sample of the _ultimate_ feature of interest. Use `hasUltimateFeatureOfInterest` if the intention is to link to the _ultimate_ feature of interest. " ;
  rdfs:comment "A relation between an Observation and the entity whose quality was observed, or between an Actuation and the entity whose property was modified, or between an act of Sampling and the entity that was sampled."@en ;
  skos:example "For example, in an Observation of the weight of a person, the FeatureOfInterest is the person and the property is its weight."@en ;
  schema:domainIncludes sosa:Actuation ;
  schema:domainIncludes sosa:ActuationCollection ;
  schema:domainIncludes sosa:Execution ;
  schema:domainIncludes sosa:Observation ;
  schema:domainIncludes sosa:ObservationCollection ;
  schema:domainIncludes sosa:Sampling ;
  schema:rangeIncludes sosa:FeatureOfInterest ;
  schema:rangeIncludes sosa:Sample ;
  owl:inverseOf sosa:isFeatureOfInterestOf ;
  rdfs:isDefinedBy sosa-core: .

sosa:hasUltimateFeatureOfInterest 
  a owl::ObjectProperty ;
  rdfs:label "has ultimate feature of interest"@en  ;
  skos:definition "A relation between an Observation and the ultimate entity whose quality was observed, or between an Actuation and the ultimate entity whose property was modified, or between an act of Sampling and the ultimate entity that was sampled. " ;
  skos:scopeNote "This is useful when the proximate feature of interest is a sample of the ultimate feature of interest, directly or transitively." ;
  rdfs:comment """should match a property chain something like this but with sosa:isSampleOf*
      owl:propertyChainAxiom ( sosa:hasFeatureOfInterest sosa:isSampleOf )""" ;
  schema:domainIncludes sosa:Actuation ;
  schema:domainIncludes sosa:ActuationCollection ;
  schema:domainIncludes sosa:Execution ;
  schema:domainIncludes sosa:Observation ;
  schema:domainIncludes sosa:ObservationCollection ;
  schema:domainIncludes sosa:Sampling ;
  schema:rangeIncludes sosa:FeatureOfInterest ;
  rdfs:isDefinedBy sosa-core: .

sosa:isFeatureOfInterestOf 
  a owl::ObjectProperty ;
  rdfs:label "is feature of interest of"@en ;
  skos:definition "A relation between a FeatureOfInterest and an Observation about it, an Actuation acting on it, or an act of Sampling that sampled it."@en ;
  rdfs:comment "A relation between a FeatureOfInterest and an Observation about it, an Actuation acting on it, or an act of Sampling that sampled it."@en ;
  schema:domainIncludes sosa:FeatureOfInterest ;
  schema:domainIncludes sosa:Sample ;
  schema:rangeIncludes sosa:Actuation ;
  schema:rangeIncludes sosa:Execution ;
  schema:rangeIncludes sosa:Observation ;
  schema:rangeIncludes sosa:Sampling ;
  owl:inverseOf sosa:hasFeatureOfInterest ;
  rdfs:isDefinedBy sosa-core: .

sosa:Property 
  a owl::Class ;
  rdfs:label "Property"@en ;
  skos:definition "An identifiable quality of a FeatureOfInterest that can be observed or acted upon. A property can apply to different features of interest."@en ;
  rdfs:comment "An identifiable quality of a FeatureOfInterest that can be observed or acted upon. A property can apply to different features of interest."@en ;
  skos:example "Cars (a feature type) all have a characteristic colour, where 'colour' is a property."@en ;
  skos:note "Concepts from existing code lists, vocabularies, and taxonomies, may be used as instances of Property"@en ;
  rdfs:isDefinedBy sosa-core: .

sosa:PropertyOfInterest 
  a owl::Class ;
  rdfs:label "Property Of Interest"@en ;
  skos:definition "An identifiable quality of a FeatureOfInterest that can be observed or acted upon. A property of interest is specific to a feature of interest. It is inherent to and cannot exist without that FeatureOfInterest."@en ;
  rdfs:comment "An identifiable quality of a FeatureOfInterest that can be observed or acted upon. A property of interest is specific to a feature of interest. It is inherent to and cannot exist without that FeatureOfInterest."@en ;
  skos:example "Abby's car has the colour red, where \"colour red\" is a property of interest of the car."@en ;
  skos:note "Properties of interest need not always be explicitly identified. It depends on the use case."@en ;
  rdfs:isDefinedBy sosa-core: .

sosa:hasProperty 
  a owl::ObjectProperty ; 
  rdfs:label "has property"@en ;
  skos:definition "Relation between an entity and a Property of that entity."@en ;
  rdfs:comment "Relation between an entity and a Property of that entity."@en ;
  schema:domainIncludes sosa:FeatureOfInterest ;
  schema:rangeIncludes sosa:Property ;
  owl:inverseOf sosa:isPropertyOf ;
  rdfs:isDefinedBy sosa-core: .

sosa:isPropertyOf 
  a owl::ObjectProperty ;
  rdfs:label "is property of"@en ;
  skos:definition "Relation between a Property and the entity it belongs to."@en ;
  rdfs:comment "Relation between a Property and the entity it belongs to."@en ;
  schema:domainIncludes sosa:Property ;
  schema:rangeIncludes sosa:FeatureOfInterest ;
  owl:inverseOf sosa:hasProperty ; 
  rdfs:isDefinedBy sosa-core: .

sosa:forProperty 
  a owl::ObjectProperty ;
  rdfs:label "for property"@en ;
  skos:definition "A relation between some aspect of an entity and a Property."@en ;
  rdfs:comment "A relation between some aspect of an entity and a Property."@en ;
  skos:example "For example, from a Sensor to the properties it can observe; from an Actuator to the properties it can act on; from a Deployment to the properties it was installed to observe or act on; from a SystemCapability to the Property the capability is described for."@en ;
  schema:rangeIncludes sosa:Property ;
  rdfs:isDefinedBy sosa-core: .


## Procedures

sosa:Procedure 
  a owl::Class ;
  rdfs:label "Procedure"@en ;
  skos:definition "A workflow, protocol, plan, algorithm, or computational method specifying how to make an Observation, create a Sample, or make a change to the state of the world (via an Actuator). A Procedure is re-usable, and might be involved in many Observations, Samplings, or Actuations. It explains the steps to be carried out to arrive at reproducible results."@en ;
  rdfs:comment "A workflow, protocol, plan, algorithm, or computational method specifying how to make an Observation, create a Sample, or make a change to the state of the world (via an Actuator). A Procedure is re-usable, and might be involved in many Observations, Samplings, or Actuations. It explains the steps to be carried out to arrive at reproducible results."@en ;
  skos:example "The measured wind speed differs depending on the height of the sensor above the surface, e.g., due to friction. Consequently, procedures for measuring wind speed define a standard height for anemometers above ground, typically 10m for meteorological measures and 2m in Agrometeorology. This definition of height, sensor placement, and so forth are defined by the Procedure."@en ;
  skos:note "Many observations may be created via the same Procedure, the same way as many tables are assembled using the same instructions (as information objects, not their concrete realization)."@en ;
  rdfs:isDefinedBy sosa-core: .

sosa:hasInput 
  a owl::ObjectProperty ;
  rdfs:label "has input"@en ;
  skos:definition "Relation between a Procedure and an Input to it."@en ;
  rdfs:comment "Relation between a Procedure and an Input to it."@en ;
  schema:domainIncludes sosa:Procedure ;
  rdfs:isDefinedBy sosa-core: .

sosa:hasOutput 
  a owl::ObjectProperty ;
  rdfs:label "has output"@en ;
  skos:definition "Relation between a Procedure and an Output of it."@en ;
  rdfs:comment "Relation between a Procedure and an Output of it."@en ;
  schema:domainIncludes sosa:Procedure ;
  rdfs:isDefinedBy sosa-core: .

sosa:usedProcedure 
  a owl::ObjectProperty ;
  rdfs:label "used procedure"@en ;
  skos:definition "A relation to link to a re-usable Procedure used in making an Observation, an Actuation, or a Sample, typically through a Sensor, Actuator or Sampler."@en ;
  rdfs:comment "A relation to link to a re-usable Procedure used in making an Observation, an Actuation, or a Sample, typically through a Sensor, Actuator or Sampler."@en ;
  schema:domainIncludes sosa:Actuation ;
  schema:domainIncludes sosa:ActuationCollection ;
  schema:domainIncludes sosa:Execution ;
  schema:domainIncludes sosa:Observation ;
  schema:domainIncludes sosa:ObservationCollection ;
  schema:domainIncludes sosa:Sampling ;
  schema:rangeIncludes sosa:Procedure ;
  rdfs:isDefinedBy sosa-core: .

## Executions

sosa:Execution 
  a owl::Class ;
  rdfs:label "Execution of a Procedure"@en ;
  skos:definition "Act of carrying out a Procedure. This class generalizes the Observation, Actuation, and Sampling classes, and is not expected to be used directly."@en ;
  rdfs:isDefinedBy sosa-core: .

sosa:hasInputValue 
  a owl::ObjectProperty ;
  rdfs:label "has input value"@en ;
  skos:definition "Assigns a value to an input defined by the Procedure that is used in an Execution (Actuation, Observation, Sampling)."@en ;
  rdfs:comment "The input value should be suitable for the input definition on the corresponding usedProcedure"@en ;
  schema:domainIncludes sosa:Actuation ;
  schema:domainIncludes sosa:Execution ;
  schema:domainIncludes sosa:Observation ;
  schema:domainIncludes sosa:Sampling ;
  rdfs:isDefinedBy sosa-core: .

sosa:hasOutputValue 
  a owl::ObjectProperty ;
  rdfs:label "has output value"@en ;
  skos:definition "Assigns a value to an output defined by the Procedure that is used in an Execution (Actuation, Observation, Sampling)."@en ;
  rdfs:comment "The output value should be suitable for the output definition on the corresponding usedProcedure"@en ;
  schema:domainIncludes sosa:Actuation ;
  schema:domainIncludes sosa:Execution ;
  schema:domainIncludes sosa:Observation ;
  schema:domainIncludes sosa:Sampling ;
  rdfs:isDefinedBy sosa-core: .

sosa:startTime 
  a owl::DatatypeProperty ;
  rdfs:label "start time"@en ;
  skos:definition """
  The instant of time when the Actuation or Observation or Sampling was initiated or tasked
  """@en ;
  rdfs:comment "The value would usually be encoded using xsd:dateTime xsd:date xsd:gYearMonth xsd:gYear"@en ;
  schema:domainIncludes sosa:Actuation ;
  schema:domainIncludes sosa:ActuationCollection ;
  schema:domainIncludes sosa:Execution ;
  schema:domainIncludes sosa:Observation ;
  schema:domainIncludes sosa:ObservationCollection ;
  schema:domainIncludes sosa:Sampling ;
  rdfs:isDefinedBy sosa-core: .

sosa:resultTime 
  a owl::DatatypeProperty ;
  rdfs:label "result time"@en ;
  skos:definition """
  The instant of time when the Actuation or Observation or Sampling was completed 
  """@en ;
  rdfs:comment "The value would usually be encoded using xsd:dateTime xsd:date xsd:gYearMonth xsd:gYear"@en ;
  schema:domainIncludes sosa:Actuation ;
  schema:domainIncludes sosa:ActuationCollection ;
  schema:domainIncludes sosa:Execution ;
  schema:domainIncludes sosa:Observation ;
  schema:domainIncludes sosa:ObservationCollection ;
  schema:domainIncludes sosa:Sampling ;
  rdfs:isDefinedBy sosa-core: .

sosa:phenomenonTime 
  a owl::ObjectProperty ;
  rdfs:label "phenomenon time"@en ;
  skos:definition """
  The time that the result of an Actuation, Observation, or Sampling applies to the FeatureOfInterest. It may be an Interval or an Instant, or some other compound TemporalEntity. 
  """@en ;
  rdfs:comment """
  The phenomenonTime is not necessarily the same as the resultTime. 
  
  In the case of Actuation, phenomenonTime should indicate the time that the actuator was active. 

  In the case of Observation, the phenomenonTime may be distant from the resultTime, for example in the case of forecasts the phenomenonTime is after the resultTime, and in historical, geological and cosmological investigations the phenomenonTime may be far in the past while the resultTime is contemporary. 

  In the case of Sampling the phenomenonTime should indicate the period during which the Sampling Procedure was active, while the resultTime may indicate when the sample comes into the posession of the operator. 
  """@en ;
  schema:domainIncludes sosa:Actuation ;
  schema:domainIncludes sosa:ActuationCollection ;
  schema:domainIncludes sosa:Execution ;
  schema:domainIncludes sosa:Observation ;
  schema:domainIncludes sosa:ObservationCollection ;
  schema:domainIncludes sosa:Sampling ;
  schema:rangeIncludes time:TemporalEntity ;
  rdfs:isDefinedBy sosa-core: .


## Result 

sosa:Result 
  a owl::Class ;
  owl:deprecated true ;
  rdfs:label "Result"@en ;
  skos:definition "The Result of an Observation, Actuation, or act of Sampling. To store an observation's simple result value one can use the hasSimpleResult property."@en ;
  skos:example "The value 20 as the height of a certain tree together with the unit, e.g., Meter."@en ;
  rdfs:isDefinedBy sosa-core: .

sosa:hasResult 
  a owl::ObjectProperty ;
  rdfs:label "has result"@en ;
  skos:definition """
  Relation linking an Actuation or Observation or act of Sampling to its result or Sample.

  In the case of an Actuation, the result is the expected value of the ActuatableProperty following the execution of the Procedure by the Actuator. 

  In the case of an Observation, the result is the value of the ObservableProperty produced by the execution of the Procedure by the Sensor. 
  
  In the case of a Sampling, the result is the Sample produced by the execution of the Procedure by the Sampler. 
  """@en ;
  schema:domainIncludes sosa:Actuation ;
  schema:domainIncludes sosa:ActuationCollection ;
  schema:domainIncludes sosa:Observation ;
  schema:domainIncludes sosa:ObservationCollection ;
  schema:domainIncludes sosa:Sampling ;
  schema:rangeIncludes sosa:Sample ;
  owl:inverseOf sosa:isResultOf ;
  rdfs:isDefinedBy sosa-core: .

sosa:isResultOf 
  a owl::ObjectProperty ;
  rdfs:label "is result of"@en ;
  skos:definition "Relation linking a Result to the Actuation or Observation or act of Sampling that created or caused it."@en ;
  schema:domainIncludes sosa:Sample ;
  schema:rangeIncludes sosa:Actuation ;
  schema:rangeIncludes sosa:Observation ;
  schema:rangeIncludes sosa:Sampling ;
  owl:inverseOf sosa:hasResult ;
  rdfs:isDefinedBy sosa-core: .

sosa:hasSimpleResult 
  a owl::DatatypeProperty ;
  rdfs:label "has simple result"@en ;
  skos:definition """
  The simple value of an Actuation or Observation.

  In the case of an Actuation, the result is the expected value of the ActuatableProperty following the execution of the Procedure by the Actuator. 

  In the case of an Observation, the result is the value of the ObservableProperty produced by the execution of the Procedure by the Sensor. 
  """@en ;
  skos:example "For instance, the values 23 or true."@en ;
  schema:domainIncludes sosa:Actuation ;
  schema:domainIncludes sosa:ActuationCollection ;
  schema:domainIncludes sosa:Observation ;
  schema:domainIncludes sosa:ObservationCollection ;
  rdfs:isDefinedBy sosa-core: .


## Systems

sosa:System 
  a owl::Class ;
  rdfs:label "System"@en ;
  skos:definition "System is a unit of abstraction for pieces of infrastructure that implement Procedures. A System may have components, its subsystems, which are other systems."@en ; 
  rdfs:comment "System is a unit of abstraction for pieces of infrastructure that implement Procedures. A System may have components, its subsystems, which are other systems."@en ; 
  rdfs:isDefinedBy sosa-core: .

sosa:hasSubSystem 
  a owl::ObjectProperty ;
  rdfs:label "has subsystem"@en ;
  skos:definition "Relation between a System and its component parts."@en ;
  rdfs:comment "Relation between a System and its component parts."@en ;
  schema:domainIncludes sosa:System ;
  schema:rangeIncludes sosa:System ;
  rdfs:isDefinedBy sosa-core: .

sosa:implements 
  a owl::ObjectProperty ;
  rdfs:label "implements"@en ;
  skos:definition "Relation between an entity that implements a Procedure in some executable way and the Procedure (an algorithm, procedure or method)."@en ;
  rdfs:comment "Relation between an entity that implements a Procedure in some executable way and the Procedure (an algorithm, procedure or method)."@en ;
  skos:example "For example, the relationship between a sensor and the scientific measuring Procedure via which it senses."@en ;
  schema:domainIncludes sosa:Actuator ;
  schema:domainIncludes sosa:Sampler ;
  schema:domainIncludes sosa:Sensor ;
  schema:rangeIncludes sosa:Procedure ;
  owl:inverseOf sosa:implementedBy ;
  rdfs:isDefinedBy sosa-core: .

sosa:implementedBy 
  a owl::ObjectProperty ;
  rdfs:label "implemented by"@en ;
  skos:definition "Relation between a Procedure (an algorithm, procedure or method) and an entity that implements that Procedure in some executable way."@en ;
  rdfs:comment "Relation between a Procedure (an algorithm, procedure or method) and an entity that implements that Procedure in some executable way."@en ;
  skos:example "For example, the relationship between a scientific measuring Procedure and a sensor that senses via that Procedure."@en ;
  schema:domainIncludes sosa:Procedure ;
  schema:rangeIncludes sosa:Actuator ;
  schema:rangeIncludes sosa:Sampler ;
  schema:rangeIncludes sosa:Sensor ;
  owl:inverseOf sosa:implements ;
  rdfs:isDefinedBy sosa-core: .


## Deployment

sosa:Deployment 
  a owl::Class ;
  rdfs:label "Deployment"@en ;
  skos:definition "Describes the Deployment of one or more assets for a particular purpose. Deployment may be done on a Platform or Host."@en ;
  rdfs:comment "Describes the Deployment of one or more assets for a particular purpose. Deployment may be done on a Platform or Host."@en ;
  skos:example "For example, a temperature Sensor deployed on a wall, or a whole network of Sensors deployed for an Observation campaign."@en ;
  rdfs:isDefinedBy sosa-core: .

sosa:deployedAsset 
  a owl::ObjectProperty ;
  rdfs:label "deployed asset"@en ;
  skos:definition "Relation between a Deployment and a deployed asset."@en ;
  rdfs:comment "Relation between a Deployment and a deployed asset."@en ;
  schema:domainIncludes sosa:Deployment ;
  rdfs:isDefinedBy sosa-core: .

sosa:deployedSystem 
  a owl::ObjectProperty ;
  rdfs:label "deployed system"@en ;
  skos:definition "Relation between a Deployment and a deployed System."@en ;
  rdfs:comment "Relation between a Deployment and a deployed System."@en ;
  owl:inverseOf sosa:hasDeployment ;
  schema:domainIncludes sosa:Deployment ;
  schema:rangeIncludes sosa:System ;
  rdfs:isDefinedBy sosa-core: .

sosa:hasDeployment 
  a owl::ObjectProperty ;
  rdfs:label "has deployment"@en ;
  skos:definition "Relation between a System and a Deployment, recording that the System is deployed in that Deployment."@en ;
  rdfs:comment "Relation between a System and a Deployment, recording that the System is deployed in that Deployment."@en ;
  owl:inverseOf sosa:deployedSystem ;
  schema:domainIncludes sosa:System ;
  schema:rangeIncludes sosa:Deployment ;
  rdfs:isDefinedBy sosa-core: .

sosa:deployedOnPlatform 
  a owl::ObjectProperty ;
  rdfs:label "deployed on platform"@en ;
  skos:definition "Relation between a Deployment and the Platform on which the Systems are deployed."@en ;
  rdfs:comment "Relation between a Deployment and the Platform on which the Systems are deployed."@en ;
  owl:inverseOf sosa:inDeployment ;
  schema:domainIncludes sosa:Deployment ;
  schema:rangeIncludes sosa:Platform ;
  rdfs:isDefinedBy sosa-core: .

sosa:inDeployment 
  a owl::ObjectProperty ;
  rdfs:label "in deployment"@en ;
  skos:definition "Relation between a Platform and a Deployment, meaning that the deployedSystems of the Deployment are hosted on the Platform."@en ;
  rdfs:comment "Relation between a Platform and a Deployment, meaning that the deployedSystems of the Deployment are hosted on the Platform."@en ;
  skos:example "For example, a relation between a buoy and a deployment of several Sensors."@en ;
  owl:inverseOf sosa:deployedOnPlatform ;
  schema:domainIncludes sosa:Platform ;
  schema:rangeIncludes sosa:Deployment ;
  rdfs:isDefinedBy sosa-core: .

## Platform 

sosa:Platform 
  a owl::Class ;
  rdfs:label "Platform or Host"@en ;
  skos:prefLabel "Platform" ;
  skos:altLabel "Host" ;
  skos:definition "A Platform is an entity that hosts other entities, particularly Sensors, Actuators, Samplers, and other Platforms."@en ;
  rdfs:comment "A Platform is an entity that hosts other entities, particularly Sensors, Actuators, Samplers, and other Platforms."@en ;
  skos:scopeNote "The INSPIRE 'Environmental Monitoring Facility' may be implemented using SOSA by the OWL/RDFS class 'Platform'" ;
  dcterms:source <https://inspire.ec.europa.eu/id/document/tg/ef> ;
  skos:example """A post, buoy, vehicle, ship, aircraft, satellite, cell-phone, human or animal may act as platforms for (technical or biological) sensors or actuators.
  An environmental monitoring facility. 
  A platform that hosts a set of sensors. 
  A team performing a survey, where each team member would be modeled as an Observer."""@en ;
  rdfs:isDefinedBy sosa-core: .

sosa:hosts 
  a owl::ObjectProperty ;
  rdfs:label "hosts"@en ;
  skos:definition "Relation between a Platform and a Sensor, Actuator, Sampler, or Platform, hosted or mounted on it."@en ;
  rdfs:comment "Relation between a Platform and a Sensor, Actuator, Sampler, or Platform, hosted or mounted on it."@en ;
  schema:domainIncludes sosa:Platform ;
  schema:rangeIncludes sosa:Actuator ;
  schema:rangeIncludes sosa:Platform ;
  schema:rangeIncludes sosa:Sampler ;
  schema:rangeIncludes sosa:Sensor ;
  owl:inverseOf sosa:isHostedBy ;
  rdfs:isDefinedBy sosa-core: .

sosa:isHostedBy 
  a owl::ObjectProperty ;
  rdfs:label "is hosted by"@en ;
  skos:definition "Relation between a Sensor, Actuator, Sampler, or Platform, and the Platform that it is mounted on or hosted by."@en ;
  rdfs:comment "Relation between a Sensor, Actuator, Sampler, or Platform, and the Platform that it is mounted on or hosted by."@en ;
  schema:domainIncludes sosa:Actuator ;
  schema:domainIncludes sosa:Platform ;
  schema:domainIncludes sosa:Sampler ;
  schema:domainIncludes sosa:Sensor ;
  schema:rangeIncludes sosa:Platform ;
  owl:inverseOf sosa:hosts ;
  rdfs:isDefinedBy sosa-core: .
